Source/DafnyCore/Verifier/Translator.ClassMembers.cs
@@ -323,7 +323,7 @@ namespace Microsoft.Dafny {
         }
       } else if (f.IsMutable) {
         // generate h[o,f]
-        oDotF = ReadHeap(c.tok, h, o, new Bpl.IdentifierExpr(c.tok, GetField(f)), TrType(f.Type));
+        oDotF = Unbox(c.tok, ReadHeap(c.tok, h, o, new Bpl.IdentifierExpr(c.tok, GetField(f))), TrType(f.Type));
         bvsTypeAxiom.Add(hVar);
         bvsTypeAxiom.Add(oVar);
         bvsAllocationAxiom.Add(hVar);
@@ -1167,7 +1167,7 @@ namespace Microsoft.Dafny {
         var bv = new Boogie.BoundVariable(p.tok, new Boogie.TypedIdent(p.tok, p.AssignUniqueName(currentDeclaration.IdGenerator), TrType(pType)));
         forallFormals.Add(bv);
         var jfArg = new Boogie.IdentifierExpr(p.tok, bv);
-        argsJF.Add(ModeledAsBoxType(p.Type) ? BoxIfUnboxed(jfArg, pType) : jfArg);
+        argsJF.Add(ModeledAsBoxType(p.Type) ? BoxIfNotNormallyBoxed(jfArg, pType) : jfArg);
         moreArgsCF.Add(new Boogie.IdentifierExpr(p.tok, bv));
       }
 
@@ -1220,7 +1220,7 @@ namespace Microsoft.Dafny {
       // The equality that is what it's all about
       var synonyms = Boogie.Expr.Eq(
         funcAppl,
-        ModeledAsBoxType(f.ResultType) ? BoxIfUnboxed(overridingFuncAppl, overridingFunction.ResultType) : overridingFuncAppl);
+        ModeledAsBoxType(f.ResultType) ? BoxIfNotNormallyBoxed(overridingFuncAppl, overridingFunction.ResultType) : overridingFuncAppl);
 
       // The axiom
       Boogie.Expr ax = BplForall(f.tok, new List<Boogie.TypeVariable>(), forallFormals, null, tr,
@@ -1409,17 +1409,16 @@ namespace Microsoft.Dafny {
       var kv = etran.TrAttributes(m.Attributes, null);
 
       var tok = m.tok;
-      var alpha = new Boogie.TypeVariable(tok, "alpha");
       var oVar = new Boogie.BoundVariable(tok, new Boogie.TypedIdent(tok, "$o", predef.RefType));
       var o = new Boogie.IdentifierExpr(tok, oVar);
-      var fVar = new Boogie.BoundVariable(tok, new Boogie.TypedIdent(tok, "$f", predef.FieldName(tok, alpha)));
+      var fVar = new Boogie.BoundVariable(tok, new Boogie.TypedIdent(tok, "$f", predef.FieldName(tok)));
       var f = new Boogie.IdentifierExpr(tok, fVar);
       var ante = Boogie.Expr.And(Boogie.Expr.Neq(o, predef.Null), etran.IsAlloced(tok, o));
 
-      // emit: assert (forall<alpha> o: ref, f: Field alpha :: o != null && $Heap[o,alloc] && (o,f) in subFrame ==> $_Frame[o,f]);
+      // emit: assert (forall o: ref, f: Field :: o != null && $Heap[o,alloc] && (o,f) in subFrame ==> $_Frame[o,f]);
       var oInCallee = InRWClause(tok, o, f, classFrameExps, etran, null, null);
       var consequent2 = InRWClause(tok, o, f, traitFrameExps, etran, null, null);
-      var q = new Boogie.ForallExpr(tok, new List<TypeVariable> { alpha }, new List<Variable> { oVar, fVar },
+      var q = new Boogie.ForallExpr(tok, new List<TypeVariable>(), new List<Variable> { oVar, fVar },
         Boogie.Expr.Imp(Boogie.Expr.And(ante, oInCallee), consequent2));
       builder.Add(Assert(m.RangeToken, q, new PODesc.TraitFrame(m.WhatKind, isModifies), kv));
     }
